Fix print of AppTerm vs AppTy (closes #4)

theories/PrettyPrinter.v
@@ -64,19 +64,19 @@ Instance PrettyName : Pretty Name :=
 Definition parens (b: bool) (s : string) :=
   if b then TkOpenPar ++ s ++ TkClosePar else s.
 
-Instance PrettyType : Pretty Typ :=
-  (fix pp barr bapp t :=
-    match t with
-    (* | TpArrowT t1 t2 => parens barr (pp true false t1 ++ TkSpace ++ TkArrow ++ TkSpace ++ pp false false t2) *)
-    | TpPi name t1 t2 => TkPi ++ TkSpace ++ pretty name ++ TkSpace
-                             ++ TkColon ++ TkSpace
-                             ++ pp false false t1 ++ TkSpace
-                             ++ TkDot ++ TkSpace ++ pp false false t2
-    | TpApp t1 ts2 => parens bapp (pp false false t1 ++ TkSpace
-                                     ++ TkTpDot ++ string_of_list_aux id (TkSpace ++ TkTpDot) (map (pp false true) ts2) 0)
-    | TpVar v => v
-    | KdStar => TkStar
-    end) false false.
+(* Instance PrettyType : Pretty Typ := *)
+(*   (fix pp barr bapp t := *)
+(*     match t with *)
+(*     (* | TpArrowT t1 t2 => parens barr (pp true false t1 ++ TkSpace ++ TkArrow ++ TkSpace ++ pp false false t2) *) *)
+(*     | TpPi name t1 t2 => TkPi ++ TkSpace ++ pretty name ++ TkSpace *)
+(*                              ++ TkColon ++ TkSpace *)
+(*                              ++ pp false false t1 ++ TkSpace *)
+(*                              ++ TkDot ++ TkSpace ++ pp false false t2 *)
+(*     | TpApp t1 ts2 => parens bapp (pp false false t1 ++ TkSpace *)
+(*                                      ++ TkTpDot ++ string_of_list_aux id (TkSpace ++ TkTpDot) (map (pp false true) ts2) 0) *)
+(*     | TpVar v => v *)
+(*     | KdStar => TkStar *)
+(*     end) false false. *)
 
 Fixpoint ppTerm' (barr bapp: bool) (t : Typ): State type_ctx string :=
     match t with
@@ -99,10 +99,24 @@ Fixpoint ppTerm' (barr bapp: bool) (t : Typ): State type_ctx string :=
                              ++ TkDot ++ TkSpace ++ t2')
       end
     | TpApp t1 ts2 =>
+      Γ <- get ;
       t1' <- ppTerm' false false t1 ;
-      let ts2' := map fst (map (fun t => ppTerm' false true t nil) ts2) in
-      pure (parens bapp (t1' ++ TkSpace ++ TkTpDot ++
-                       string_of_list_aux id (TkSpace ++ TkTpDot) ts2' 0))
+      let ppApp (t: Typ) :=
+          (match t with
+           | TpVar n =>
+             match ctx_find n Γ with
+             | None => ""
+             | Some t =>
+               match t with
+               | KdStar => TkTpDot
+               | _ => ""
+               end
+             end
+           | _ => ""
+          end) ++ fst (ppTerm' false true t nil) in
+      (* let ts2' := map fst (map (fun t => ppTerm' false true t nil) ts2) in *)
+      let ts2' := (map ppApp ts2) in
+      pure (parens bapp (t1' ++ TkSpace ++ string_of_list_aux id (TkSpace) ts2' 0))
     | TpVar v => pure v
     | KdStar => pure TkStar
     end.
@@ -162,14 +176,13 @@ Fixpoint removeParams (data_name : Var) params_count (t: Typ) :=
   | _ => t
   end.
 
-Definition ppctor params_count data_name ctor :=
+Definition ppctor params_count (Γ: type_ctx) data_name ctor :=
   match ctor with
   | Ctr cname ty =>
-    let '(no_bindings_t, Γ) := removeBindings ty params_count nil in
+    let '(no_bindings_t, Γ') := removeBindings ty params_count nil in
     let no_params_t := removeParams data_name params_count no_bindings_t in
-    TkPipe ++ TkSpace ++ cname ++ TkSpace ++ TkColon ++ TkSpace ++ ppTerm no_params_t Γ
+    TkPipe ++ TkSpace ++ cname ++ TkSpace ++ TkColon ++ TkSpace ++ ppTerm no_params_t (List.app Γ Γ')
   end.
-
 
 Instance PrettyParams : Pretty Params :=
   fix pp params :=
@@ -177,34 +190,56 @@ Instance PrettyParams : Pretty Params :=
     | nil => ""
     | cons (n, t) ps =>
       TkSpace ++ TkOpenPar ++ n ++ TkSpace
-              ++ TkColon ++ TkSpace ++ pretty t
+              ++ TkColon ++ TkSpace ++ (ppTerm t nil)
               ++ TkClosePar ++ pp ps
     end.
 
-Definition ppDatatype (name : Var) (params: Params) (kind : Typ) (ctors : list Ctor) :=
+Definition ppDatatype (name : Var) (params: Params) (kind : Typ) (ctors : list Ctor) Γ :=
   TkData ++ TkSpace ++ name ++ pretty params ++ TkSpace ++ TkColon ++ TkSpace
-          ++ pretty kind ++ TkSpace ++ TkAssgn ++ TkCR
-          ++ string_of_list (ppctor (List.length params) name) ctors 1 ++ TkDot.
+          ++ ppTerm kind Γ ++ TkSpace ++ TkAssgn ++ TkCR
+          ++ string_of_list (ppctor (List.length params) Γ name) ctors 1 ++ TkDot.
 
 
 Instance PrettyAssgn : Pretty Assgn :=
   fun asgn =>
     match asgn with
     | AssgnType name t => name ++ TkSpace ++ TkAssgn
-                              ++ TkSpace ++ pretty t
-                              ++ TkDot ++ TkCR
+                              ++ TkSpace ++ ppTerm t nil
+                              ++ TkDot
     | AssgnTerm name t => TkNotImpl
     end.
 
-Instance PrettyCmd : Pretty Cmd :=
-  fun c =>
+(* Instance PrettyCmd : Pretty Cmd := *)
+(*   fun c => *)
+(*     match c with *)
+(*     | CmdAssgn def => pretty def ++ TkCR *)
+(*     | CmdData (DefData name params kind ctors)  => ppDatatype name params kind ctors ++ TkCR *)
+(*     end. *)
+
+Definition ppCmd (c: Cmd): State type_ctx string :=
     match c with
-    | CmdAssgn def => pretty def ++ TkCR
-    | CmdData (DefData name params kind ctors)  => ppDatatype name params kind ctors ++ TkCR
+    | CmdAssgn def => pure (pretty def)
+    | CmdData (DefData name params kind ctors)  =>
+      Γ <- get ;
+      let s := ppDatatype name params kind ctors Γ ++ TkCR in
+      put ((name, kind) :: Γ) ;;
+      pure s
     end.
 
+Fixpoint ppProgram' (p : Program) : State type_ctx string :=
+  match p with
+  | nil => pure ""
+  | c :: cs =>
+    c' <- ppCmd c;
+    cs' <- ppProgram' cs;
+    pure (c' ++ TkCR ++ cs')
+  end.
+
+(* Instance PrettyProgram : Pretty Program := *)
+  (* fun p => string_of_list pretty p 0. *)
+
 Instance PrettyProgram : Pretty Program :=
-  fun p => string_of_list pretty p 0.
+  fun p => fst (ppProgram' p nil).
 
 Instance PrettyOption {A} {x: Pretty A}: Pretty (option A) :=
   fun o =>
