tests/Extraction.v
@@ -43,6 +43,7 @@ Quote Recursively Definition nat_syntax := nat.
 Quote Recursively Definition list_syntax := list.
 Quote Recursively Definition option_syntax := option.
 Quote Recursively Definition vector_syntax := Vectors.Vector.t.
+Quote Recursively Definition nat_syntax := le.
 (* We are finally ready to extract the programs we want *)
 Extraction "main.hs" PrettyProgram denoteCoq
            nat_syntax list_syntax option_syntax vector_syntax.
