theories/Ast.v
@@ -24,7 +24,6 @@ Module Ced.
   Inductive Typ : Type :=
   | TpPi (_: Name) (_: Typ) (_: Typ)
   | TpApp (_: Typ) (_: list Typ)
-  | TpArrowT (_: Typ) (_: Typ)
   | TpVar (_: Var)
   | KdStar
   .
