theories/demo.v
@@ -8,7 +8,15 @@ Require Import Coquedille.PrettyPrinter.
 
 Require Import String.
 Require Import List. Import ListNotations.
-Require Import Vectors.Vector.
+
+Inductive Vec (A : Type) : nat -> Type :=
+| vnil : Vec A 0
+| vcons : A -> forall (n : nat), Vec A n -> Vec A (S n)
+.
+
+Quote Recursively Definition vector_syntax := Vec.
+Eval compute in (pretty (denoteCoq vector_syntax)).
+
 
 Quote Recursively Definition nat_syntax := nat.
 Quote Recursively Definition option_syntax := option.
@@ -16,12 +24,13 @@ Quote Recursively Definition option_syntax := option.
 Quote Recursively Definition list_syntax :=
 ltac:(let t := eval compute in list in exact t).
 
-Quote Recursively Definition vector_syntax := t.
+(* Quote Recursively Definition vector_syntax := Vector.t. *)
 
 
 Inductive mytry : Type :=
 | foo
 | bar : ((nat -> nat) -> (nat -> list nat)) -> mytry
+| asdf : Vec nat 3 -> mytry
 .
 
 Quote Recursively Definition x1 := (mytry).
@@ -34,6 +43,9 @@ Eval compute in (pretty (denoteCoq vector_syntax)).
 
 Definition x' := nat.
 Definition x := x'.
+
+Quote Recursively Definition le_syntax := le.
+Eval compute in (pretty (denoteCoq le_syntax)).
 
 Inductive myDep (A : Type) : x -> Type :=
 | mynil : myDep A 0
@@ -192,6 +204,7 @@ Inductive mydata (A B C: Type) (D : nat -> Type) :=
 | baz' : forall x, D x -> mydata A B C D
 .
 
+
 Quote Recursively Definition mydata_syntax := mydata.
 Print mydata_syntax.
 (* mydata_syntax =  *)
@@ -259,3 +272,205 @@ Print tst_syntax.
 Definition denotetst := (denoteCoq tst_syntax).
 Eval compute in denotetst.
 Eval compute in (pretty denotetst).
+
+Inductive tst_data (A B C : Type) :=
+| tst_ctor : C -> A -> B -> tst_data B C B -> tst_data A B C
+.
+
+Quote Recursively Definition tstdata_syntax := tst_data.
+Definition xxx := denoteCoq tstdata_syntax.
+Eval compute in xxx.
+(* tstdata_syntax =  *)
+(* ([InductiveDecl "Top.tst_data" *)
+(*     {| *)
+(*     ind_finite := Finite; *)
+(*     ind_npars := 3; *)
+(*     ind_params := [{| *)
+(*                    decl_name := nNamed "C"; *)
+(*                    decl_body := None; *)
+(*                    decl_type := tSort *)
+(*                                   (Universe.make'' *)
+(*                                      (Level.Level "Top.136", false) *)
+(*                                      []) |}; *)
+(*                   {| *)
+(*                   decl_name := nNamed "B"; *)
+(*                   decl_body := None; *)
+(*                   decl_type := tSort *)
+(*                                  (Universe.make'' *)
+(*                                     (Level.Level "Top.135", false) *)
+(*                                     []) |}; *)
+(*                   {| *)
+(*                   decl_name := nNamed "A"; *)
+(*                   decl_body := None; *)
+(*                   decl_type := tSort *)
+(*                                  (Universe.make'' *)
+(*                                     (Level.Level "Top.134", false) *)
+(*                                     []) |}]; *)
+(*     ind_bodies := [{| *)
+(*                    ind_name := "tst_data"; *)
+(*                    ind_type := tProd (nNamed "A") *)
+(*                                  (tSort *)
+(*                                     (Universe.make'' *)
+(*                                        (Level.Level "Top.134", *)
+(*                                        false) [])) *)
+(*                                  (tProd (nNamed "B") *)
+(*                                     (tSort *)
+(*                                        (Universe.make'' *)
+(*                                           (Level.Level "Top.135", *)
+(*                                           false) [])) *)
+(*                                     (tProd (nNamed "C") *)
+(*                                        (tSort *)
+(*                                           (Universe.make'' *)
+(*                                            ( *)
+(*                                            Level.Level "Top.136", *)
+(*                                            false) [])) *)
+(*                                        (tSort *)
+(*                                           (Universe.make'' *)
+(*                                            ( *)
+(*                                            Level.Level "Top.134", *)
+(*                                            false) *)
+(*                                            [ *)
+(*                                            ( *)
+(*                                            Level.Level "Top.135", *)
+(*                                            false); *)
+(*                                            ( *)
+(*                                            Level.Level "Top.136", *)
+(*                                            false)])))); *)
+(*                    ind_kelim := [InProp; InSet; InType]; *)
+(*                    ind_ctors := [("tst_ctor", *)
+(*                                  tProd (nNamed "A") *)
+(*                                    (tSort *)
+(*                                       (Universe.make'' *)
+(*                                          (Level.Level "Top.134", *)
+(*                                          false) [])) *)
+(*                                    (tProd (nNamed "B") *)
+(*                                       (tSort *)
+(*                                          (Universe.make'' *)
+(*                                            ( *)
+(*                                            Level.Level "Top.135", *)
+(*                                            false) [])) *)
+(*                                       (tProd  *)
+(*                                          (nNamed "C") *)
+(*                                          (tSort *)
+(*                                            (Universe.make'' *)
+(*                                            ( *)
+(*                                            Level.Level "Top.136", *)
+(*                                            false) [])) *)
+(*                                          (tProd nAnon  *)
+(*                                            (tRel 0) *)
+(*                                            (tProd nAnon  *)
+(*                                            (tRel 3) *)
+(*                                            (tProd nAnon  *)
+(*                                            (tRel 3) *)
+(*                                            (tApp  *)
+(*                                            (tRel 6) *)
+(*                                            [tRel 5; tRel 4; tRel 3])))))), *)
+(*                                  3)]; *)
+(*                    ind_projs := [] |}]; *)
+(*     ind_universes := Monomorphic_ctx *)
+(*                        (LevelSetProp.of_list *)
+(*                           [Level.Level "Top.136"; *)
+(*                           Level.Level "Top.135"; *)
+(*                           Level.Level "Top.134"], *)
+(*                        ConstraintSet.empty) |}], *)
+(* tInd {| inductive_mind := "Top.tst_data"; inductive_ind := 0 |} []) *)
+(*      : program *)
+
+
+
+Eval compute in (pretty (denoteCoq tstdata_syntax)).
+
+Inductive tst_data2 (A : Type) (D : nat -> Type ) :=
+| tst_ctor2 : A -> tst_data2 A D
+.
+
+Quote Recursively Definition tstdata2_syntax := tst_data2.
+Definition xx := denoteCoq tstdata2_syntax.
+Eval compute in xx.
+(* tstdata2_syntax =  *)
+(* ([InductiveDecl "Top.tst_data2" *)
+(*     {| *)
+(*     ind_finite := Finite; *)
+(*     ind_npars := 2; *)
+(*     ind_params := [{| *)
+(*                    decl_name := nNamed "D"; *)
+(*                    decl_body := None; *)
+(*                    decl_type := tProd nAnon *)
+(*                                   (tSort *)
+(*                                      (Universe.make'' *)
+(*                                         (Level.lProp, false) [])) *)
+(*                                   (tSort *)
+(*                                      (Universe.make'' *)
+(*                                         (Level.Level "Top.163", *)
+(*                                         false) [])) |}; *)
+(*                   {| *)
+(*                   decl_name := nNamed "A"; *)
+(*                   decl_body := None; *)
+(*                   decl_type := tSort *)
+(*                                  (Universe.make'' *)
+(*                                     (Level.Level "Top.162", false) *)
+(*                                     []) |}]; *)
+(*     ind_bodies := [{| *)
+(*                    ind_name := "tst_data2"; *)
+(*                    ind_type := tProd (nNamed "A") *)
+(*                                  (tSort *)
+(*                                     (Universe.make'' *)
+(*                                        (Level.Level "Top.162", *)
+(*                                        false) [])) *)
+(*                                  (tProd (nNamed "D") *)
+(*                                     (tProd nAnon *)
+(*                                        (tSort *)
+(*                                           (Universe.make'' *)
+(*                                            (Level.lProp, false) [])) *)
+(*                                        (tSort *)
+(*                                           (Universe.make'' *)
+(*                                            ( *)
+(*                                            Level.Level "Top.163", *)
+(*                                            false) []))) *)
+(*                                     (tSort *)
+(*                                        (Universe.make'' *)
+(*                                           (Level.Level "Top.162", *)
+(*                                           false) []))); *)
+(*                    ind_kelim := [InProp; InSet; InType]; *)
+(*                    ind_ctors := [("tst_ctor2", *)
+(*                                  tProd (nNamed "A") *)
+(*                                    (tSort *)
+(*                                       (Universe.make'' *)
+(*                                          (Level.Level "Top.162", *)
+(*                                          false) [])) *)
+(*                                    (tProd (nNamed "D") *)
+(*                                       (tProd nAnon *)
+(*                                          (tSort *)
+(*                                            (Universe.make'' *)
+(*                                            (Level.lProp, false) [])) *)
+(*                                          (tSort *)
+(*                                            (Universe.make'' *)
+(*                                            ( *)
+(*                                            Level.Level "Top.163", *)
+(*                                            false) []))) *)
+(*                                       (tProd nAnon  *)
+(*                                          (tRel 1) *)
+(*                                          (tApp  *)
+(*                                            (tRel 3) *)
+(*                                            [tRel 2; tRel 1]))), 1)]; *)
+(*                    ind_projs := [] |}]; *)
+(*     ind_universes := Monomorphic_ctx *)
+(*                        (LevelSetProp.of_list *)
+(*                           [Level.Level "Top.163"; *)
+(*                           Level.Level "Top.162"], *)
+(*                        ConstraintSet.empty) |}], *)
+(* tInd {| inductive_mind := "Top.tst_data2"; inductive_ind := 0 |} []) *)
+(*      : program *)
+
+Eval compute in (pretty (denoteCoq tstdata2_syntax)).
+(*      = "data nat : ★ = *)
+(*   | O : nat *)
+(*   | S : nat ➔ nat. *)
+
+(* data tst_data2 (A : ★) (D : nat ➔ ★) : ★ = *)
+(*   | tst_ctor2 : dummy ➔ A ·dummy ·D. *)
+
+(* _ = tst_data2. *)
+
+(* " *)
+(*      : string *)
